SystemF2Data: finish liftTT_wfT lemma

proof/DDC/Language/SystemF2/Ty.v
@@ -4,33 +4,6 @@ Require Export DDC.Language.SystemF2.TyLift.
 Require Export DDC.Language.SystemF2.TySubst.
 
 
-(* Well formed types are closed under the given kind environment. *)
-Inductive wfT (kn: nat) : ty -> Prop :=
- | WfT_TVar 
-   :  forall ki
-   ,  ki < kn
-   -> wfT kn (TVar ki)
-
- | WfT_TCon
-   :  forall n
-   ,  wfT kn (TCon n)
-
- | WfT_TForall
-   :  forall t
-   ,  wfT (S kn) t
-   -> wfT kn (TForall t)
-
- | WfT_TApp
-   :  forall t1 t2
-   ,  wfT kn t1 -> wfT kn t2
-   -> wfT kn (TApp t1 t2).
-Hint Constructors wfT.
-
-
-(* Closed types are well formed under an empty environment. *)
-Definition closedT (tt: ty) : Prop
- := wfT O tt.
-Hint Unfold closedT.
 
 
 
